Encoder proof; [skip ci]

src/Primitive/BooleanVSTSpecEncoder.v
@@ -69,6 +69,76 @@ Definition bool_der_encode_spec : ident * funspec :=
 Definition Gprog := ltac:(with_library prog [der_write_tags_spec; 
                                                bool_der_encode_spec]).
 
+Definition if_post1 cb_p sptr_p v_bool_value v_erval gv 
+           td_p tag_mode tag app_p td b := 
+  PROP(cb_p = nullval \/ cb_p <> nullval)
+  LOCAL(temp _t'6 (Vint (Int.repr 2)); 
+        temp _t'1 (Vint (Int.repr (encoded {| encoded := 2 |}))); 
+        temp _st sptr_p; lvar _bool_value tuchar v_bool_value; 
+        lvar _erval (Tstruct _asn_enc_rval_s noattr) v_erval; 
+        gvars gv; temp __res Vundef; temp _td td_p; 
+        temp _sptr sptr_p; 
+        temp _tag_mode (Vint (Int.repr tag_mode)); 
+        temp _tag (Vint (Int.repr tag)); temp _cb cb_p; 
+        temp _app_key app_p) 
+  SEP(data_at_ Tsh type_descriptor_s td_p; 
+      data_at_ Tsh tvoid app_p; func_ptr cb_spec cb_p; 
+      data_at Tsh tuchar 
+              (Vbyte (match execErrW (bool_encoder td b) [] with 
+                      | Some v => last v (Byte.repr (-1)) 
+                      | None => (Byte.repr (-1)) 
+                      end)) v_bool_value;
+      data_at Tsh enc_rval_s 
+              (match evalErrW (bool_encoder td b) [] with 
+               | Some v => construct_enc_rval (encoded v) td sptr_p 
+               | None => construct_enc_rval (-1) td sptr_p 
+               end) v_erval;
+      data_at Tsh tint (Vint (int_of_bool b)) sptr_p; 
+      valid_pointer cb_p).
+
+Definition if_post2 b (cb_p app_p v_bool_value : val) cb_spec 
+           cb_p v_bool_value v_erval:= 
+  PROP(b = true \/ b = false)
+  LOCAL(temp _cb cb_p; temp _app_key app_p; 
+        lvar _bool_value tuchar v_bool_value; 
+        temp _t'2 (Vint (Int.repr (if b then 255 else 0))))
+  SEP(data_at_ Tsh tvoid app_p; func_ptr cb_spec cb_p;
+      data_at Tsh tuchar (Vint (int_of_bool b)) v_bool_value; 
+      field_at Tsh (Tstruct _asn_enc_rval_s noattr) (DOT _encoded) 
+               (Vint (Int.repr 2)) v_erval;
+      field_at Tsh (Tstruct _asn_enc_rval_s noattr) (DOT _failed_type)
+               (default_val (tptr (Tstruct _asn_TYPE_descriptor_s noattr))) 
+               v_erval;
+      field_at Tsh (Tstruct _asn_enc_rval_s noattr) (DOT _structure_ptr)
+               (default_val (tptr tvoid)) v_erval).
+
+Definition loop_inv_post sptr_p v_bool_value v_erval gv td_p tag_mode tag
+  cb_p app_p cb_spec td b :=
+  PROP()
+  LOCAL(temp _t'6 (Vint (Int.repr 2)); 
+        temp _t'1 (Vint (Int.repr (encoded {| encoded := 2 |}))); 
+        temp _st sptr_p; lvar _bool_value tuchar v_bool_value; 
+        lvar _erval (Tstruct _asn_enc_rval_s noattr) v_erval; 
+        gvars gv; temp __res Vundef; temp _td td_p; 
+        temp _sptr sptr_p; 
+        temp _tag_mode (Vint (Int.repr tag_mode)); 
+        temp _tag (Vint (Int.repr tag)); temp _cb cb_p; 
+        temp _app_key app_p) 
+  SEP(data_at_ Tsh type_descriptor_s td_p; 
+      data_at_ Tsh tvoid app_p; func_ptr cb_spec cb_p; 
+      data_at Tsh tuchar 
+              (Vbyte (match execErrW (bool_encoder td b) [] with 
+                      | Some v => last v (Byte.repr (-1)) 
+                      | None => (Byte.repr (-1)) 
+                      end)) v_bool_value;
+      data_at Tsh enc_rval_s 
+              (match evalErrW (bool_encoder td b) [] with 
+               | Some v => construct_enc_rval (encoded v) td sptr_p 
+               | None => construct_enc_rval (-1) td sptr_p 
+               end) v_erval;
+      data_at Tsh tint (Vint (int_of_bool b)) sptr_p; 
+      valid_pointer cb_p).
+
 Theorem bool_der_encode : semax_body Vprog Gprog 
                                      (normalize_function 
                                         f_BOOLEAN_encode_der composites) 
@@ -83,46 +153,42 @@ Proof.
   forward.
   forward.
   forward_if; [contradiction|].
-  forward_if (cb_p = nullval).
+  forward_if (if_post1 cb_p sptr_p v_bool_value v_erval gv td_p tag_mode tag
+              app_p td b).
   * (* if(cb) = true *)
     forward.
     (* bool_value = *st ? 0xff : 0; /* 0xff mandated by DER */ *)
-    forward_if (PROP(b = true \/ b = false)
-                LOCAL(temp _t'2 (Vint (Int.repr (if b then 255 else 0))))
-                SEP()).
+    forward_if (if_post2 b cb_p app_p v_bool_value cb_spec cb_p 
+                         v_bool_value v_erval).
     - (* if(b) = true *)
-      forward.
-      entailer!.
+      forward; unfold if_post2; entailer!.
     - (* if(b) = false *)
-      forward.
-      entailer!.
-    -
+      forward; unfold if_post2; entailer!.
+    - unfold if_post2.
       Intros.
-      destruct b eqn:B.
-      admit.
+      forward.
+      (* Definition cb_spec : funspec := 
+         WITH buf_addr : val, buf : val, size : Z, app_addr : val, app_key : val *)
+      (* forward_call (v_bool_value, Vint (int_of_bool b), 1, app_p, Vundef). *)
       admit.
   * (* if(cb) = false *)
+    forward; unfold if_post1; entailer!.
+  * unfold if_post1.
     forward.
-    entailer!.
-  *
     forward.
-    forward.
-    forward_loop 
-      (PROP() LOCAL() SEP()) 
-      (* This must be a postcondition of whole function *)
-      break:(PROP() 
-             LOCAL()
-             SEP(field_at Tsh (Tstruct _asn_enc_rval_s noattr) (DOT _encoded) 
-                          (Vint (Int.add (Int.repr 2) (Int.repr 1))) v_erval; 
-                 field_at Tsh (Tstruct _asn_enc_rval_s noattr) (DOT _failed_type) 
-                          (default_val 
-                             (tptr (Tstruct _asn_TYPE_descriptor_s noattr))) 
-                          v_erval)).
+    forward_loop (loop_inv_post sptr_p v_bool_value v_erval gv td_p tag_mode tag
+                                cb_p app_p cb_spec td b)
+                 break: (loop_inv_post sptr_p v_bool_value v_erval gv td_p 
+                                       tag_mode tag cb_p app_p cb_spec td b).
+    unfold loop_inv_post.
     - entailer!.
-    - admit.
-    - admit.
-     
-
-  
+    - unfold loop_inv_post.
+      forward.
+      forward.
+      admit.
+    - 
+      unfold loop_inv_post.
+      admit.
+Admitted.     
 
 End Boolean_der_encode_primitive.
